src/temporal_logic/scheduling.lean
@@ -1,0 +1,122 @@
+
+import .lemmas
+
+import data.set.basic
+
+import util.data.minimum
+import util.function
+import util.logic
+
+open temporal function predicate
+
+local infix ` ≃ `:75 := v_eq
+local attribute [instance] classical.prop_decidable
+universe u
+
+namespace temporal.scheduling
+section scheduling
+
+parameter {evt : Type u}
+parameter Γ : cpred
+parameters {f : evt → ℕ} (Hinj : injective f)
+parameter r : tvar (set evt)
+parameter Hr : Γ ⊢ ◻-(r ≃ (∅ : set evt))
+parameter [nonempty evt]
+
+abbreviation SCHED  (s : tvar evt) :=
+◻(s ∊ r) ⋀
+∀∀ (e : evt),
+  ◻◇(↑e ∊ r) ⟶
+  ◻◇(s ≃ ↑e ⋀ ↑e ∊ r)
+
+section implementation
+
+parameter q : tvar (evt → ℕ)
+parameter cur : tvar ℕ
+
+infixr ` |+| `:80 := lifted₂ has_add.add
+
+parameter cur_Spec : Γ ⊢ cur ≃ ↑0 ⋀ ◻(⊙cur ≃ cur |+| ↑1)
+
+def next : tvar $ (evt → ℕ) → (evt → ℕ) :=
+[| r cur, λ q : evt → ℕ, q |]
+
+abbreviation Spec :=
+q ≃ ↑f ⋀ ◻(⊙q ≃ next q)
+
+parameter Hq : Γ ⊢ Spec
+
+noncomputable def select : tvar evt :=
+[| q r , inv q (↓ i, inv q i ∈ r)  |]
+
+include Hq Hinj
+
+def q_injective
+: Γ ⊢ ◻(⟨injective⟩ ! q) :=
+begin [temporal]
+  cases Hq with Hq Hq',
+  t_induction!,
+  explicit' { cc },
+  { henceforth at Hq',
+    explicit' { admit } },
+end
+
+open set
+include Hr
+def sched_inv
+: Γ ⊢ ◻(select ∊ r) :=
+begin [temporal]
+  have Hq := temporal.scheduling.q_injective,
+  persistent, henceforth at *,
+  explicit' [select]
+  { apply @minimum_mem _ _ { i | inv q i ∈ r },
+    simp [not_eq_empty_iff_exists],
+    apply exists_imp_exists_simpl q,
+    have := inv_is_left_inverse_of_injective Hq, simp [left_inverse] at this,
+    conv in (inv q (q _))
+    { rw [inv_is_left_inverse_of_injective Hq], },
+    rw [← ne_empty_iff_exists_mem], exact Hr },
+end
+
+def sched_fairness (e : evt)
+: Γ ⊢ ◻◇(↑e ∊ r) ⟶ ◻◇(select ≃ ↑e ⋀ ↑e ∊ r) :=
+begin [temporal]
+  cases Hq with _ Hq, persistent,
+  apply inf_often_induction' (q ↑ e) ; intro q₀,
+  { admit },
+  { henceforth at ⊢ Hq,
+    simp, intros hreq hq₀,
+    apply next_entails_eventually,
+    -- simp [select,next],
+    explicit' [select,next]
+    { by_cases h : e ∈ r' ; admit } },
+end
+
+def correct_sched
+: Γ ⊢ SCHED select :=
+begin [temporal]
+  split,
+  { apply temporal.scheduling.sched_inv, },
+  { intro, apply temporal.scheduling.sched_fairness },
+end
+
+end implementation
+
+set_option trace.app_builder true
+
+include f Hinj
+lemma scheduler
+  (hr : Γ ⊢ ◻-(r ≃ (∅ : set evt)))
+: Γ ⊢ (∃∃ s, SCHED s) :=
+begin [temporal]
+  have := witness ↑(0 : ℕ) ( ↑(has_add.add 1) : tvar (ℕ → ℕ)) Γ,
+  cases this with cur Hcur,
+  have := witness (f : tvar (evt → ℕ)) (next r cur) Γ,
+  cases this with q Hq,
+  existsi select r q,
+  apply correct_sched _ Hinj _ hr,
+  exact Hq,
+end
+
+end scheduling
+end temporal.scheduling
