Makefile
@@ -1,13 +1,24 @@
 
-.PHONY: all clean lines
+.PHONY: all clean lines profile
 
 LEAN_OPT =
+SRC = $(shell git ls-files | grep "\\.lean")
+PROF = $(SRC:.lean=.lean.test_suite.out)
+
+profile:
+	leanpkg build -- --profile --test-suite
+
+# %.prof.txt: %.lean
+# %.lean.test_suite.out: %.lean
+# 	lean $^ --profile --test-suite
 
 all:
 	leanpkg build
 
 clean:
 	/usr/bin/find . -name "*.olean" -delete
+	/usr/bin/find . -name "*.lean.test_suite.out" -delete
+	/usr/bin/find . -name "*.lean.status" -delete
 
 lines:
 	wc `git ls-files | grep .lean`
